theories/ambiguity.v
@@ -1,0 +1,283 @@
+From Coq Require Import ssreflect.
+From stdpp Require Import prelude.
+From ambig Require Import grammar sub_derive.
+
+Section ambiguity.
+
+  Variable Σ N : Type.
+  Implicit Type t s T : tree Σ N.
+
+  (* similarity *)
+
+  (* assume input trees have same root and word *)
+
+  Definition similar (t1 t2 : tree Σ N) : Prop :=
+    match t1, t2 with
+    | ε_tree _, ε_tree _ => True
+    | token_tree R1 tk1, token_tree R2 tk2 => tk1 = tk2
+    | unary_tree R1 t1, unary_tree R2 t2 => root t1 = root t2
+    | binary_tree R1 tA1 tB1, binary_tree R2 tA2 tB2 =>
+        root tA1 = root tA2 ∧ root tB1 = root tB2 ∧ word tA1 = word tA2
+    | _, _ => False
+    end.
+
+  Lemma similar_refl :
+    Reflexive similar.
+  Proof.
+    move => t.
+    destruct t => //=.
+  Qed.
+
+  (* local ambiguity *)
+
+  Variable G : grammar Σ N.
+
+  Context `{EqDecision Σ}.
+  Context `{EqDecision N}.
+
+  Definition local_amb A w : Prop :=
+    ∃ H h, reachable G (A, w) (H, h) ∧
+      ∃ t1 t2, t1 ▷ H ={G}=> h ∧ t2 ▷ H ={G}=> h ∧ ¬ (similar t1 t2).
+
+  Ltac invert H := inversion H; subst; clear H.
+
+  (* first direction : local ambiguous -> derivation ambiguous *)
+
+  Fixpoint subst T t s : option (tree Σ N) :=
+    match T with
+    | unary_tree A t1 =>
+      if bool_decide (T = t) then Some s else
+      t1' ← subst t1 t s; Some (unary_tree A t1')
+    | binary_tree A tl tr =>
+      if bool_decide (T = t) then Some s else
+      match subst tl t s with
+      | Some tl' => Some (binary_tree A tl' tr)
+      | None => tr' ← subst tr t s; Some (binary_tree A tl tr')
+      end
+    | _ => if bool_decide (T = t) then Some s else None
+    end.
+
+  Ltac push_bind :=
+    match goal with 
+    | [ |- context [ ?x ≫= _ ] ] => destruct x; simpl
+    end.
+
+  Lemma subst_Some T t s :
+    subtree t T → is_Some (subst T t s).
+  Proof.
+    intros Ht.
+    induction T => /=.
+    1: apply subtree_ε_inv in Ht.
+    2: apply subtree_token_inv in Ht.
+    3: apply subtree_unary_inv in Ht.
+    4: apply subtree_binary_inv in Ht.
+    all: repeat case_bool_decide.
+    all: repeat case_match.
+    all: repeat push_bind.
+    all: naive_solver.
+  Qed.
+
+  Lemma subst_id T t s :
+    subst T t s = Some T → s = t.
+  Proof.
+    induction T => /=.
+    all: repeat case_bool_decide => //=.
+    all: repeat case_match.
+    all: repeat push_bind.
+    all: naive_solver.
+  Qed.
+
+  Lemma subst_witness T t s T' A w H h :
+    T ▷ A ={G}=> w →
+    t ▷ H ={G}=> h →
+    s ▷ H ={G}=> h →
+    subst T t s = Some T' →
+    T' ▷ A ={G}=> w.
+  Proof.
+    intros [? [? ?]] [? [? ?]] Hs.
+    generalize dependent A.
+    generalize dependent w.
+    generalize dependent T'.
+    induction T => T' w ? A ? /=.
+    all: repeat case_bool_decide => //=.
+    all: repeat case_match.
+    all: repeat push_bind.
+    all: inversion 1; subst => //.
+    - invert H2.
+      have [Hr [Hw ?]] : t0 ▷ (root T) ={ G }=> (word T) by naive_solver.
+      repeat split => //. econstructor => //. by rewrite Hr. by rewrite Hw.
+    - invert H2.
+      have [Hr [Hw ?]] : t0 ▷ (root T1) ={ G }=> (word T1) by naive_solver.
+      repeat split => //. simpl. by rewrite Hw.
+      econstructor => //. by rewrite Hr. by rewrite Hw.
+    - invert H2.
+      have [Hr [Hw ?]] : t0 ▷ (root T2) ={ G }=> (word T2) by naive_solver.
+      repeat split => //. simpl. by rewrite Hw.
+      econstructor => //. by rewrite Hr. by rewrite Hw.
+  Qed.
+
+  Lemma subst_subtree T t s T' :
+    subst T t s = Some T' → subtree s T'.
+  Proof.
+    generalize dependent T'.
+    induction T => T' /=.
+    all: repeat case_bool_decide => //=.
+    all: repeat case_match.
+    all: repeat push_bind.
+    all: inversion 1; subst => //.
+    all: apply rtc_r with (y := t0); [naive_solver | constructor].
+  Qed.
+
+  Lemma local_amb_implies_derive_amb A w :
+    local_amb A w → derive_amb G A w.
+  Proof.
+    intros [H [h [Hr [t1 [t2 [Ht1 [Ht2 Hnot]]]]]]].
+    apply reachable_spec in Hr; last by exists t1.
+    specialize (Hr _ Ht1) as [t [Ht Hsub]].
+    edestruct (subst_Some _ _ t2 Hsub) as [t' ?].
+    exists t', t. split; last split.
+    - eapply subst_witness. apply Ht. apply Ht1. apply Ht2. eauto.
+    - done.
+    - intros <-.
+      have ? : t2 = t1 by eapply subst_id; eauto.
+      subst. apply Hnot, similar_refl.
+  Qed.
+
+  (* second direction : derivation ambiguous -> local ambiguous *)
+
+  (* diff two trees with same root and sentence *)
+  Fixpoint diff t1 t2 : option (tree Σ N * tree Σ N) :=
+    match t1, t2 with
+    | ε_tree _, ε_tree _ => None
+    | token_tree _ _, token_tree _ _ =>
+      (* tokens must be eq, so no diff *)
+      None
+    | unary_tree _ t1', unary_tree _ t2' =>
+      (* sentences must be eq, so just compare root *)
+      if bool_decide (root t1' = root t2')
+      then diff t1' t2'
+      else Some (t1, t2)
+    | binary_tree _ tl1 tr1, binary_tree _ tl2 tr2 =>
+      if bool_decide (root tl1 = root tl2 ∧ root tr1 = root tr2 ∧ word tl1 = word tl2)
+      then
+        match diff tl1 tl2 with
+        | Some p => Some p
+        | None => diff tr1 tr2
+        end
+      else Some (t1, t2)
+    | _, _ => Some (t1, t2)
+    end.
+
+  Lemma diff_None t1 t2 :
+    root t1 = root t2 →
+    word t1 = word t2 →
+    t1 = t2 ↔ diff t1 t2 = None.
+  Proof.
+    intros. split.
+    - intros <-.
+      induction t1 => //=.
+      + case_bool_decide => //. by apply IHt1.
+      + case_bool_decide => //=.
+        * rewrite IHt1_1 => //. rewrite IHt1_2 => //.
+        * exfalso. naive_solver.
+    - generalize dependent t2.
+      induction t1 => t2.
+      all: destruct t2 => Hr Hw Hdiff //=.
+      1,2: naive_solver.
+      + simpl in Hr; subst.
+        simpl in Hdiff. case_bool_decide => //.
+        erewrite IHt1; eauto.
+      + simpl in Hr; subst.
+        simpl in Hdiff. case_bool_decide => //.
+        case_match => //.
+        erewrite (IHt1_1 t2_1).
+        erewrite (IHt1_2 t2_2).
+        all: eauto; naive_solver.
+  Qed.
+
+  Lemma diff_Some_inv t1 t2 t1' t2' :
+    root t1 = root t2 →
+    word t1 = word t2 →
+    diff t1 t2 = Some (t1', t2') →
+    root t1' = root t2' ∧ word t1' = word t2'.
+  Proof.
+    generalize dependent t2.
+    induction t1 => t2.
+    all: destruct t2 => //= -> Hw Hdiff.
+    all: inversion Hdiff; subst; clear Hdiff => //.
+    - case_bool_decide.
+      * eapply IHt1; eauto.
+      * inversion H0; subst; clear H0. done.
+    - case_bool_decide; first case_match.
+      * naive_solver.
+      * destruct H as [? [? ?]]. eapply (IHt1_2 t2_2); eauto.
+        rewrite H2 in Hw. by eapply app_inv_head_iff.
+      * naive_solver.
+  Qed.
+
+  Lemma diff_result_not_similar t1 t2 t1' t2' :
+    diff t1 t2 = Some (t1', t2') → ¬ (similar t1' t2').
+  Proof.
+    generalize dependent t2.
+    induction t1 => t2.
+    all: destruct t2 => //= Hdiff.
+    all: inversion Hdiff; subst; clear Hdiff.
+    all: try naive_solver.
+    - case_bool_decide; naive_solver.
+    - case_bool_decide; first case_match; naive_solver.
+  Qed.
+
+  Lemma diff_result_subtree t1 t2 t1' t2' :
+    diff t1 t2 = Some (t1', t2') → subtree t1' t1 ∧ subtree t2' t2.
+  Proof.
+    generalize dependent t2.
+    induction t1 => t2.
+    all: destruct t2 => //= Hdiff.
+    all: inversion Hdiff; subst; clear Hdiff.
+    all: try by split; constructor.
+    - case_bool_decide.
+      * edestruct IHt1; eauto. split; etrans; eauto.
+        all: apply rtc_once; constructor.
+      * inversion H0; subst. split; by constructor.
+    - case_bool_decide; first case_match.
+      * edestruct (IHt1_1 t2_1); eauto; try congruence. split; etrans; eauto.
+        all: apply rtc_once; constructor.
+      * edestruct (IHt1_2 t2_2); eauto. split; etrans; eauto.
+        all: apply rtc_once; constructor.
+      * inversion H0; subst. split; by constructor.
+  Qed.
+
+  Lemma derive_amb_implies_local_amb A w :
+    derive_amb G A w → local_amb A w.
+  Proof.
+    intros [t1 [t2 [[Hr1 [Hw1 ?]] [[? [? ?]] ?]]]].
+    have [[t1' t2'] Hdiff] : is_Some (diff t1 t2).
+    { apply not_eq_None_Some. intros Hcontra. apply diff_None in Hcontra => //.
+      all: congruence. }
+    have [Hsub1 Hsub2] := (diff_result_subtree _ _ _ _ Hdiff).
+    have Ht1' : t1' ▷ root t1' ={G}=> word t1'.
+    { repeat split. eapply subtree_valid; eauto. }
+    exists (root t1'), (word t1'). split.
+    - apply reachable_spec; first by exists t1'.
+      intros t' Ht'.
+      edestruct (subst_Some _ _ t' Hsub1) as [T ?].
+      exists T. split; last eapply subst_subtree; eauto.
+      eapply subst_witness. 2: apply Ht1'. 2: apply Ht'. 2: eauto.
+      by repeat split.
+    - exists t1', t2'.
+      have [? ?] : root t1' = root t2' ∧ word t1' = word t2'.
+      { eapply diff_Some_inv; last eauto. all: congruence. }
+      repeat split => //. eapply subtree_valid; eauto.
+      eapply diff_result_not_similar; eauto.
+  Qed.
+
+  (* To sum up *)
+
+  Theorem derive_amb_iff_local_amb A w :
+    derive_amb G A w ↔ local_amb A w.
+  Proof.
+    split; [ apply derive_amb_implies_local_amb
+           | apply local_amb_implies_derive_amb ].
+  Qed.
+
+End ambiguity.
